feat: refactor ArmState by making fields private
Note that this breaks the build,
so this commit will be reverted.
We will revive it for the next PR where we correctly reorganize projections,
and move other dependencies that use projections (e.g. read_mem/write_mem)
into Arm/ArmState.lean

Arm/State.lean
@@ -121,27 +121,35 @@ structure PState where
   v : BitVec 1
 deriving DecidableEq, Repr
 
-def PState.default : PState where 
+def PState.default : PState where
   n := 0#1
   z := 0#1
   c := 0#1
   v := 0#1
 
-instance : Inhabited PState where 
+instance : Inhabited PState where
   default := PState.default
 
+/--
+Note that we mark all fields except `program` as private, since we expect users
+to interact with these via a uniform API provided by `r` and `w`,
+or the higher level `{read|write}_<field_name>` functions that are sugar over `r` and `w`.
+
+This allows us to prove theorems about (non)interference once in terms of `r` and `w`,
+and reuse these for automation.
+-/
 @[ext]
 structure ArmState where
   -- General-purpose registers: register 31 is the stack pointer.
-  gpr        : Store (BitVec 5) (BitVec 64)
+  private gpr        : Store (BitVec 5) (BitVec 64)
   -- SIMD/floating-point registers
-  sfp        : Store (BitVec 5) (BitVec 128)
+  private sfp        : Store (BitVec 5) (BitVec 128)
   -- Program Counter
-  pc         : BitVec 64
+  private pc         : BitVec 64
   -- PState
-  pstate     : PState
+  private pstate     : PState
   -- Memory: maps 64-bit addresses to bytes
-  mem        : Store (BitVec 64) (BitVec 8)
+  private mem        : Store (BitVec 64) (BitVec 8)
   -- Program: maps 64-bit addresses to 32-bit instructions.
   -- Note that we have the following assumption baked into our machine model:
   -- the program is always disjoint from the rest of the memory.
@@ -151,10 +159,10 @@ structure ArmState where
   -- non-None value when some irrecoverable error is encountered
   -- (e.g., an unimplemented instruction is hit). Any reasoning or
   -- execution based off an erroneous state is invalid.
-  error      : StateError
+  private error      : StateError
 deriving Repr
 
-def ArmState.default : ArmState where 
+def ArmState.default : ArmState where
   gpr := .const 0
   sfp := .const 0
   pc := 0#64
@@ -163,7 +171,7 @@ def ArmState.default : ArmState where
   error := .None
   program := []
 
-instance : Inhabited ArmState where 
+instance : Inhabited ArmState where
   default := .default
 
 ---- Basic State Accessors and Updaters (except memory) ----
