Proofs/Experiments/Abs.lean
@@ -7,7 +7,10 @@ Author(s): Shilpi Goel, Siddharth Bhat
 The goal is to prove that this program implements absolute value correctly.
 -/
 
-def int_abs_program : Program :=
+
+namespace Abs
+
+def program : Program :=
   def_program
    [(0x4005d0#64, 0x2a0003e1#32), --  mov w1, w0
     (0x4005d4#64, 0x131f7c00#32), --  asr w0, w0, #31
@@ -15,5 +18,15 @@ def int_abs_program : Program :=
     (0x4005dc#64, 0x4a000020#32), --  eor w0, w1, w0
     (0x4005e0#64, 0xd65f03c0#32)] --  ret
 
-def intAbs (x : BitVec 32) : BitVec 32 := BitVec.ofNat 32 x.toInt.natAbs
+def spec (x : BitVec 32) : BitVec 32 := BitVec.ofNat 32 x.toInt.natAbs
 
+theorem correct
+  {s0 sf : ArmState}
+  (h_s0_pc : read_pc s0 = 0x4005d0#64)
+  (h_s0_program : s0.program = int_abs_program)
+  (h_s0_err : read_err s0 = StateError.None)
+  (h_run : sf = run int_abs_program.length s0) :
+  read_gpr 32 0 sf = spec (read_gpr 32 0 s0) ∧
+  read_err sf = StateError.None := by sorry
+
+end Abs
