Proofs/Experiments/Memcpy.lean
@@ -5,9 +5,18 @@ Author(s): Shilpi Goel, Siddharth Bhat
 
 The goal is to prove that this program implements memcpy correctly.
 -/
-import Arm 
+import Arm
 
-def mem_copy_program : Program :=
+def ArmState.x (n : Nat) : ArmState → BitVec 64
+| s => read_gpr 64 n s
+
+def ArmState.x0 := ArmState.x 0
+def ArmState.x1 := ArmState.x 1
+def ArmState.x2 := ArmState.x 2
+
+
+namespace Memcpy
+def program : Program :=
   def_program
     [
      /- 00000000000008e0 <mem_copy>:                         -/
@@ -22,5 +31,38 @@ def mem_copy_program : Program :=
      (0x8f8#64, 0xd65f03c0#32)   /- ret                      -/
     ]
 
+def spec (x y : BitVec 32) : BitVec 32 :=
+  if BitVec.slt y x then x else y
 
 
+structure Correct (s0 sf : ArmState) : Prop where
+  /-- The destination in the final state is a copy of the source in the initial state. -/
+  hdest : read_mem_bytes s0.x0.toNat x₂ sf = read_mem_bytes s0.x0.toNat x₁ s0
+  /-- All memory regions that do not overlap with the destination are unchanged. -/
+  hdisjoint : ∀ (n : Nat)
+    (addr : BitVec 64)
+    (hsep : mem_separate s0.x2 (s0.x2 + s0.x0 - 1) addr (addr + (BitVec.ofNat _ n) - 1)),
+      read_mem_bytes n addr sf = read_mem_bytes n addr s0
+  herr : read_err sf  = .None
+
+/-
+Note that the theorem also holds when src = dest, but does *not* hold
+when src and dest overlap.
+
+num bytes to be copied is x0.
+src address is in x1.
+dest address is in x2.
+-/
+theorem correct_separate
+  {s0 sf : ArmState}
+  (h_s0_pc : read_pc s0 = 0x4005d0#64)
+  (h_s0_program : s0.program = int_abs_program)
+  (h_s0_err : read_err s0 = StateError.None)
+  (h_run : sf = run program.length s0)
+  (hx₀ : x₀ = read_gpr 64 0 s0)
+  (hx₁ : x₁ = read_gpr 64 1 s0)
+  (hx₂ : x₂ = read_gpr 64 2 s0)
+  (h_s0_mem : mem_separate  x₁ (x₀ + x₁ - 1) x₂ (x₂ + x₀ - 1)) : -- TODO: These are closed intervals.
+  Correct s0 sf := sorry
+
+end Memcpy
